Handle implicit arguments uniformly inside Coq printer.

src/printer/coq.ml
@@ -73,7 +73,7 @@ let print_implicit_tv_binder fmt tv =
 
 let print_ne_params fmt stv =
   Stv.iter
-    (fun tv -> fprintf fmt "@ %a" print_tv_binder tv)
+    (fun tv -> fprintf fmt "@ %a" print_implicit_tv_binder tv)
     stv
 
 let print_ne_params_list fmt ltv =
@@ -373,15 +373,6 @@ let ls_ty_vars ls =
   let ty_vars_value = option_fold Ty.ty_freevars Stv.empty ls.ls_value in
   (ty_vars_args, ty_vars_value, Stv.union ty_vars_args ty_vars_value)
 
-let print_implicits fmt ls ty_vars_args ty_vars_value all_ty_params =
-  if not (Stv.is_empty all_ty_params) then
-    begin
-      let need_context = not (Stv.subset ty_vars_value ty_vars_args) in
-      if need_context then fprintf fmt "Set Contextual Implicit.@\n";
-      fprintf fmt "Implicit Arguments %a.@\n" print_ls ls;
-      if need_context then fprintf fmt "Unset Contextual Implicit.@\n"
-    end
-
 (*
 
   copy of old user scripts
@@ -646,8 +637,12 @@ let print_data_decl info fmt (ts,csl) =
     (print_list newline (print_constr info ts)) csl;
   List.iter
     (fun (cs,_) ->
-      let ty_vars_args, ty_vars_value, all_ty_params = ls_ty_vars cs in
-      print_implicits fmt cs ty_vars_args ty_vars_value all_ty_params)
+      let _, _, all_ty_params = ls_ty_vars cs in
+      if not (Stv.is_empty all_ty_params) then
+        let print fmt tv = fprintf fmt "[%a]" print_tv tv in
+        fprintf fmt "Implicit Arguments %a [%a].@\n"
+           print_ls cs
+           (print_list space print) ts.ts_args)
     csl;
   fprintf fmt "@\n"
 
@@ -662,7 +657,7 @@ let print_ls_type ?(arrow=false) info fmt ls =
   | Some ty -> print_ty info fmt ty
 
 let print_param_decl ~prev info fmt ls =
-  let ty_vars_args, ty_vars_value, all_ty_params = ls_ty_vars ls in
+  let _, _, all_ty_params = ls_ty_vars ls in
   begin if info.realization then
     match prev with
       | Some (Query (_,Notation,c)) ->
@@ -679,7 +674,6 @@ let print_param_decl ~prev info fmt ls =
         (print_arrow_list (print_ty info)) ls.ls_args
         (print_ls_type ~arrow:(ls.ls_args <> []) info) ls.ls_value
   end;
-  print_implicits fmt ls ty_vars_args ty_vars_value all_ty_params;
   fprintf fmt "@\n"
 
 let print_param_decl ~prev info fmt ls =
@@ -687,7 +681,7 @@ let print_param_decl ~prev info fmt ls =
     (print_param_decl ~prev info fmt ls; forget_tvs ())
 
 let print_logic_decl info fmt (ls,ld) =
-  let ty_vars_args, ty_vars_value, all_ty_params = ls_ty_vars ls in
+  let _, _, all_ty_params = ls_ty_vars ls in
   let vl,e = open_ls_defn ld in
   fprintf fmt "(* Why3 assumption *)@\n@[<hov 2>Definition %a%a%a: %a :=@ %a.@]@\n"
     print_ls ls
@@ -696,7 +690,6 @@ let print_logic_decl info fmt (ls,ld) =
     (print_ls_type info) ls.ls_value
     (print_expr info) e;
   List.iter forget_var vl;
-  print_implicits fmt ls ty_vars_args ty_vars_value all_ty_params;
   fprintf fmt "@\n"
 
 let print_logic_decl info fmt d =
@@ -718,26 +711,25 @@ let print_recursive_decl info fmt (ls,ld) =
   List.iter forget_var vl
 
 let print_recursive_decl info fmt dl =
-  fprintf fmt "(* Why3 assumption *)@\nSet Implicit Arguments.@\n";
+  fprintf fmt "(* Why3 assumption *)@\n";
   print_list_delim
     ~start:(fun fmt () -> fprintf fmt "@[<hov 2>Fixpoint ")
     ~stop:(fun fmt () -> fprintf fmt ".@\n")
     ~sep:(fun fmt () -> fprintf fmt "@\n@[<hov 2>with ")
     (fun fmt d -> print_recursive_decl info fmt d; forget_tvs ())
     fmt dl;
-  fprintf fmt "Unset Implicit Arguments.@\n@\n"
+  fprintf fmt "@\n"
 
 let print_ind info fmt (pr,f) =
   fprintf fmt "@[<hov 4>| %a : %a@]" print_pr pr (print_fmla info) f
 
 let print_ind_decl info s fmt (ps,bl) =
-  let ty_vars_args, ty_vars_value, all_ty_params = ls_ty_vars ps in
+  let _, _, all_ty_params = ls_ty_vars ps in
   fprintf fmt "(* Why3 assumption *)@\n@[<hov 2>%s %a%a : %a -> Prop :=@ @[<hov>%a@].@]@\n"
     (match s with Ind -> "Inductive" | Coind -> "CoInductive")
      print_ls ps print_implicit_params all_ty_params
     (print_arrow_list (print_ty info)) ps.ls_args
      (print_list newline (print_ind info)) bl;
-  print_implicits fmt ps ty_vars_args ty_vars_value all_ty_params;
   fprintf fmt "@\n"
 
 let print_ind_decl info s fmt d =
