examples/programs/bellman_ford/bf_WP_BellmanFord_key_lemma_2_1.v
@@ -7,179 +7,133 @@ Require int.Int.
 (* Why3 assumption *)
 Definition unit  := unit.
 
-Parameter qtmark : Type.
-
-Parameter at1: forall (a:Type), a -> qtmark -> a.
-Implicit Arguments at1.
-
-Parameter old: forall (a:Type), a -> a.
-Implicit Arguments old.
-
-(* Why3 assumption *)
-Definition implb(x:bool) (y:bool): bool := match (x,
-  y) with
-  | (true, false) => false
-  | (_, _) => true
-  end.
-
 Parameter map : forall (a:Type) (b:Type), Type.
 
-Parameter get: forall (a:Type) (b:Type), (map a b) -> a -> b.
-Implicit Arguments get.
+Parameter get: forall {a:Type} {b:Type}, (map a b) -> a -> b.
 
-Parameter set: forall (a:Type) (b:Type), (map a b) -> a -> b -> (map a b).
-Implicit Arguments set.
+Parameter set: forall {a:Type} {b:Type}, (map a b) -> a -> b -> (map a b).
 
-Axiom Select_eq : forall (a:Type) (b:Type), forall (m:(map a b)),
+Axiom Select_eq : forall {a:Type} {b:Type}, forall (m:(map a b)),
   forall (a1:a) (a2:a), forall (b1:b), (a1 = a2) -> ((get (set m a1 b1)
   a2) = b1).
 
-Axiom Select_neq : forall (a:Type) (b:Type), forall (m:(map a b)),
+Axiom Select_neq : forall {a:Type} {b:Type}, forall (m:(map a b)),
   forall (a1:a) (a2:a), forall (b1:b), (~ (a1 = a2)) -> ((get (set m a1 b1)
   a2) = (get m a2)).
 
-Parameter const: forall (b:Type) (a:Type), b -> (map a b).
-Set Contextual Implicit.
-Implicit Arguments const.
-Unset Contextual Implicit.
+Parameter const: forall {a:Type} {b:Type}, b -> (map a b).
 
-Axiom Const : forall (b:Type) (a:Type), forall (b1:b) (a1:a),
+Axiom Const : forall {a:Type} {b:Type}, forall (b1:b) (a1:a),
   ((get (const b1:(map a b)) a1) = b1).
 
 (* Why3 assumption *)
 Inductive list (a:Type) :=
   | Nil : list a
   | Cons : a -> (list a) -> list a.
-Set Contextual Implicit.
-Implicit Arguments Nil.
-Unset Contextual Implicit.
-Implicit Arguments Cons.
+Implicit Arguments Nil [[a]].
+Implicit Arguments Cons [[a]].
 
 (* Why3 assumption *)
-Set Implicit Arguments.
-Fixpoint length (a:Type)(l:(list a)) {struct l}: Z :=
+Fixpoint length {a:Type}(l:(list a)) {struct l}: Z :=
   match l with
   | Nil => 0%Z
   | (Cons _ r) => (1%Z + (length r))%Z
   end.
-Unset Implicit Arguments.
 
-Axiom Length_nonnegative : forall (a:Type), forall (l:(list a)),
+Axiom Length_nonnegative : forall {a:Type}, forall (l:(list a)),
   (0%Z <= (length l))%Z.
 
-Axiom Length_nil : forall (a:Type), forall (l:(list a)),
+Axiom Length_nil : forall {a:Type}, forall (l:(list a)),
   ((length l) = 0%Z) <-> (l = (Nil :(list a))).
 
 Parameter set1 : forall (a:Type), Type.
 
-Parameter mem: forall (a:Type), a -> (set1 a) -> Prop.
-Implicit Arguments mem.
+Parameter mem: forall {a:Type}, a -> (set1 a) -> Prop.
 
 (* Why3 assumption *)
-Definition infix_eqeq (a:Type)(s1:(set1 a)) (s2:(set1 a)): Prop :=
+Definition infix_eqeq {a:Type}(s1:(set1 a)) (s2:(set1 a)): Prop :=
   forall (x:a), (mem x s1) <-> (mem x s2).
-Implicit Arguments infix_eqeq.
 
-Axiom extensionality : forall (a:Type), forall (s1:(set1 a)) (s2:(set1 a)),
+Axiom extensionality : forall {a:Type}, forall (s1:(set1 a)) (s2:(set1 a)),
   (infix_eqeq s1 s2) -> (s1 = s2).
 
 (* Why3 assumption *)
-Definition subset (a:Type)(s1:(set1 a)) (s2:(set1 a)): Prop := forall (x:a),
+Definition subset {a:Type}(s1:(set1 a)) (s2:(set1 a)): Prop := forall (x:a),
   (mem x s1) -> (mem x s2).
-Implicit Arguments subset.
 
-Axiom subset_trans : forall (a:Type), forall (s1:(set1 a)) (s2:(set1 a))
+Axiom subset_trans : forall {a:Type}, forall (s1:(set1 a)) (s2:(set1 a))
   (s3:(set1 a)), (subset s1 s2) -> ((subset s2 s3) -> (subset s1 s3)).
 
-Parameter empty: forall (a:Type), (set1 a).
-Set Contextual Implicit.
-Implicit Arguments empty.
-Unset Contextual Implicit.
+Parameter empty: forall {a:Type}, (set1 a).
 
 (* Why3 assumption *)
-Definition is_empty (a:Type)(s:(set1 a)): Prop := forall (x:a), ~ (mem x s).
-Implicit Arguments is_empty.
+Definition is_empty {a:Type}(s:(set1 a)): Prop := forall (x:a), ~ (mem x s).
 
-Axiom empty_def1 : forall (a:Type), (is_empty (empty :(set1 a))).
+Axiom empty_def1 : forall {a:Type}, (is_empty (empty :(set1 a))).
 
-Parameter add: forall (a:Type), a -> (set1 a) -> (set1 a).
-Implicit Arguments add.
+Parameter add: forall {a:Type}, a -> (set1 a) -> (set1 a).
 
-Axiom add_def1 : forall (a:Type), forall (x:a) (y:a), forall (s:(set1 a)),
+Axiom add_def1 : forall {a:Type}, forall (x:a) (y:a), forall (s:(set1 a)),
   (mem x (add y s)) <-> ((x = y) \/ (mem x s)).
 
-Parameter remove: forall (a:Type), a -> (set1 a) -> (set1 a).
-Implicit Arguments remove.
+Parameter remove: forall {a:Type}, a -> (set1 a) -> (set1 a).
 
-Axiom remove_def1 : forall (a:Type), forall (x:a) (y:a) (s:(set1 a)), (mem x
+Axiom remove_def1 : forall {a:Type}, forall (x:a) (y:a) (s:(set1 a)), (mem x
   (remove y s)) <-> ((~ (x = y)) /\ (mem x s)).
 
-Axiom subset_remove : forall (a:Type), forall (x:a) (s:(set1 a)),
+Axiom subset_remove : forall {a:Type}, forall (x:a) (s:(set1 a)),
   (subset (remove x s) s).
 
-Parameter union: forall (a:Type), (set1 a) -> (set1 a) -> (set1 a).
-Implicit Arguments union.
+Parameter union: forall {a:Type}, (set1 a) -> (set1 a) -> (set1 a).
 
-Axiom union_def1 : forall (a:Type), forall (s1:(set1 a)) (s2:(set1 a)) (x:a),
+Axiom union_def1 : forall {a:Type}, forall (s1:(set1 a)) (s2:(set1 a)) (x:a),
   (mem x (union s1 s2)) <-> ((mem x s1) \/ (mem x s2)).
 
-Parameter inter: forall (a:Type), (set1 a) -> (set1 a) -> (set1 a).
-Implicit Arguments inter.
+Parameter inter: forall {a:Type}, (set1 a) -> (set1 a) -> (set1 a).
 
-Axiom inter_def1 : forall (a:Type), forall (s1:(set1 a)) (s2:(set1 a)) (x:a),
+Axiom inter_def1 : forall {a:Type}, forall (s1:(set1 a)) (s2:(set1 a)) (x:a),
   (mem x (inter s1 s2)) <-> ((mem x s1) /\ (mem x s2)).
 
-Parameter diff: forall (a:Type), (set1 a) -> (set1 a) -> (set1 a).
-Implicit Arguments diff.
+Parameter diff: forall {a:Type}, (set1 a) -> (set1 a) -> (set1 a).
 
-Axiom diff_def1 : forall (a:Type), forall (s1:(set1 a)) (s2:(set1 a)) (x:a),
+Axiom diff_def1 : forall {a:Type}, forall (s1:(set1 a)) (s2:(set1 a)) (x:a),
   (mem x (diff s1 s2)) <-> ((mem x s1) /\ ~ (mem x s2)).
 
-Axiom subset_diff : forall (a:Type), forall (s1:(set1 a)) (s2:(set1 a)),
+Axiom subset_diff : forall {a:Type}, forall (s1:(set1 a)) (s2:(set1 a)),
   (subset (diff s1 s2) s1).
 
-Parameter choose: forall (a:Type), (set1 a) -> a.
-Implicit Arguments choose.
+Parameter choose: forall {a:Type}, (set1 a) -> a.
 
-Axiom choose_def : forall (a:Type), forall (s:(set1 a)), (~ (is_empty s)) ->
+Axiom choose_def : forall {a:Type}, forall (s:(set1 a)), (~ (is_empty s)) ->
   (mem (choose s) s).
 
-Parameter all: forall (a:Type), (set1 a).
-Set Contextual Implicit.
-Implicit Arguments all.
-Unset Contextual Implicit.
+Parameter cardinal: forall {a:Type}, (set1 a) -> Z.
 
-Axiom all_def : forall (a:Type), forall (x:a), (mem x (all :(set1 a))).
-
-Parameter cardinal: forall (a:Type), (set1 a) -> Z.
-Implicit Arguments cardinal.
-
-Axiom cardinal_nonneg : forall (a:Type), forall (s:(set1 a)),
+Axiom cardinal_nonneg : forall {a:Type}, forall (s:(set1 a)),
   (0%Z <= (cardinal s))%Z.
 
-Axiom cardinal_empty : forall (a:Type), forall (s:(set1 a)),
+Axiom cardinal_empty : forall {a:Type}, forall (s:(set1 a)),
   ((cardinal s) = 0%Z) <-> (is_empty s).
 
-Axiom cardinal_add : forall (a:Type), forall (x:a), forall (s:(set1 a)),
+Axiom cardinal_add : forall {a:Type}, forall (x:a), forall (s:(set1 a)),
   (~ (mem x s)) -> ((cardinal (add x s)) = (1%Z + (cardinal s))%Z).
 
-Axiom cardinal_remove : forall (a:Type), forall (x:a), forall (s:(set1 a)),
+Axiom cardinal_remove : forall {a:Type}, forall (x:a), forall (s:(set1 a)),
   (mem x s) -> ((cardinal s) = (1%Z + (cardinal (remove x s)))%Z).
 
-Axiom cardinal_subset : forall (a:Type), forall (s1:(set1 a)) (s2:(set1 a)),
+Axiom cardinal_subset : forall {a:Type}, forall (s1:(set1 a)) (s2:(set1 a)),
   (subset s1 s2) -> ((cardinal s1) <= (cardinal s2))%Z.
 
-Axiom cardinal1 : forall (a:Type), forall (s:(set1 a)),
+Axiom cardinal1 : forall {a:Type}, forall (s:(set1 a)),
   ((cardinal s) = 1%Z) -> forall (x:a), (mem x s) -> (x = (choose s)).
 
-Parameter nth: forall (a:Type), Z -> (set1 a) -> a.
-Implicit Arguments nth.
+Parameter nth: forall {a:Type}, Z -> (set1 a) -> a.
 
-Axiom nth_injective : forall (a:Type), forall (s:(set1 a)) (i:Z) (j:Z),
+Axiom nth_injective : forall {a:Type}, forall (s:(set1 a)) (i:Z) (j:Z),
   ((0%Z <= i)%Z /\ (i < (cardinal s))%Z) -> (((0%Z <= j)%Z /\
   (j < (cardinal s))%Z) -> (((nth i s) = (nth j s)) -> (i = j))).
 
-Axiom nth_surjective : forall (a:Type), forall (s:(set1 a)) (x:a), (mem x
+Axiom nth_surjective : forall {a:Type}, forall (s:(set1 a)) (x:a), (mem x
   s) -> exists i:Z, ((0%Z <= i)%Z /\ (i < (cardinal s))%Z) -> (x = (nth i
   s)).
 
@@ -202,38 +156,34 @@ Axiom s_in_graph : (mem s vertices).
 Axiom vertices_cardinal_pos : (0%Z < (cardinal vertices))%Z.
 
 (* Why3 assumption *)
-Set Implicit Arguments.
-Fixpoint infix_plpl (a:Type)(l1:(list a)) (l2:(list a)) {struct l1}: (list
+Fixpoint infix_plpl {a:Type}(l1:(list a)) (l2:(list a)) {struct l1}: (list
   a) :=
   match l1 with
   | Nil => l2
   | (Cons x1 r1) => (Cons x1 (infix_plpl r1 l2))
   end.
-Unset Implicit Arguments.
 
-Axiom Append_assoc : forall (a:Type), forall (l1:(list a)) (l2:(list a))
+Axiom Append_assoc : forall {a:Type}, forall (l1:(list a)) (l2:(list a))
   (l3:(list a)), ((infix_plpl l1 (infix_plpl l2
   l3)) = (infix_plpl (infix_plpl l1 l2) l3)).
 
-Axiom Append_l_nil : forall (a:Type), forall (l:(list a)), ((infix_plpl l
+Axiom Append_l_nil : forall {a:Type}, forall (l:(list a)), ((infix_plpl l
   (Nil :(list a))) = l).
 
-Axiom Append_length : forall (a:Type), forall (l1:(list a)) (l2:(list a)),
+Axiom Append_length : forall {a:Type}, forall (l1:(list a)) (l2:(list a)),
   ((length (infix_plpl l1 l2)) = ((length l1) + (length l2))%Z).
 
 (* Why3 assumption *)
-Set Implicit Arguments.
-Fixpoint mem1 (a:Type)(x:a) (l:(list a)) {struct l}: Prop :=
+Fixpoint mem1 {a:Type}(x:a) (l:(list a)) {struct l}: Prop :=
   match l with
   | Nil => False
   | (Cons y r) => (x = y) \/ (mem1 x r)
   end.
-Unset Implicit Arguments.
 
-Axiom mem_append : forall (a:Type), forall (x:a) (l1:(list a)) (l2:(list a)),
+Axiom mem_append : forall {a:Type}, forall (x:a) (l1:(list a)) (l2:(list a)),
   (mem1 x (infix_plpl l1 l2)) <-> ((mem1 x l1) \/ (mem1 x l2)).
 
-Axiom mem_decomp : forall (a:Type), forall (x:a) (l:(list a)), (mem1 x l) ->
+Axiom mem_decomp : forall {a:Type}, forall (x:a) (l:(list a)), (mem1 x l) ->
   exists l1:(list a), exists l2:(list a), (l = (infix_plpl l1 (Cons x l2))).
 
 (* Why3 assumption *)
@@ -248,8 +198,8 @@ Axiom path_right_extension : forall (x:vertex) (y:vertex) (z:vertex) (l:(list
 
 Axiom path_right_inversion : forall (x:vertex) (z:vertex) (l:(list vertex)),
   (path x l z) -> (((x = z) /\ (l = (Nil :(list vertex)))) \/
-  exists y:vertex, exists lqt:(list vertex), (path x lqt y) /\ ((edge y z) /\
-  (l = (infix_plpl lqt (Cons y (Nil :(list vertex))))))).
+  exists y:vertex, exists l':(list vertex), (path x l' y) /\ ((edge y z) /\
+  (l = (infix_plpl l' (Cons y (Nil :(list vertex))))))).
 
 Axiom path_trans : forall (x:vertex) (y:vertex) (z:vertex) (l1:(list vertex))
   (l2:(list vertex)), (path x l1 y) -> ((path y l2 z) -> (path x
@@ -265,14 +215,12 @@ Axiom path_decomposition : forall (x:vertex) (y:vertex) (z:vertex) (l1:(list
 Parameter weight: vertex -> vertex -> Z.
 
 (* Why3 assumption *)
-Set Implicit Arguments.
 Fixpoint path_weight(l:(list vertex)) (dst:vertex) {struct l}: Z :=
   match l with
   | Nil => 0%Z
   | (Cons x Nil) => (weight x dst)
   | (Cons x ((Cons y _) as r)) => ((weight x y) + (path_weight r dst))%Z
   end.
-Unset Implicit Arguments.
 
 Axiom path_weight_right_extension : forall (x:vertex) (y:vertex) (l:(list
   vertex)), ((path_weight (infix_plpl l (Cons x (Nil :(list vertex))))
@@ -344,8 +292,8 @@ Axiom long_path_decomposition : forall (l:(list vertex)) (v:vertex), (path s
   l3))))))).
 
 Axiom simple_path : forall (v:vertex) (l:(list vertex)), (path s l v) ->
-  exists lqt:(list vertex), (path s lqt v) /\
-  ((length lqt) < (cardinal vertices))%Z.
+  exists l':(list vertex), (path s l' v) /\
+  ((length l') < (cardinal vertices))%Z.
 
 (* Why3 assumption *)
 Definition negative_cycle(v:vertex): Prop := (mem v vertices) /\
@@ -398,14 +346,13 @@ Axiom Total : forall (x:t) (y:t), (le x y) \/ (le y x).
 (* Why3 assumption *)
 Inductive ref (a:Type) :=
   | mk_ref : a -> ref a.
-Implicit Arguments mk_ref.
+Implicit Arguments mk_ref [[a]].
 
 (* Why3 assumption *)
-Definition contents (a:Type)(v:(ref a)): a :=
+Definition contents {a:Type}(v:(ref a)): a :=
   match v with
   | (mk_ref x) => x
   end.
-Implicit Arguments contents.
 
 (* Why3 assumption *)
 Definition t1 (a:Type) := (ref (set1 a)).
@@ -460,7 +407,7 @@ unfold le, add1.
 right; ae.
 intros h _. 
 absurd ((length (Cons v0 l) <= 0)%Z); auto.
-unfold length; fold length.
+unfold length; fold @length.
 generalize (length_nonneg _ l).
 omega.
 clear n hn. intros n hn IH.
@@ -468,7 +415,7 @@ intros vi l hl hpath.
 destruct (path_right_inversion v vi l hpath) as [(eq1,eq2)|(y,(l',(y1,(y2,y3))))].
 subst; simpl. ae.
 assert (hl': (length l = length l' + 1)%Z).
-generalize (Append_length _ l' (Cons y Nil)).
+generalize (Append_length l' (Cons y Nil)).
 ae.
 subst l. rewrite path_weight_right_extension.
 rewrite hl' in hl. clear hl'.
