examples/programs/edit_distance/edit_distance_Word_first_last_1.v
@@ -2,56 +2,37 @@
 (* Beware! Only edit allowed sections below    *)
 Require Import ZArith.
 Require Import Rbase.
-Axiom Max_is_ge : forall (x:Z) (y:Z), (x <= (Zmax x y))%Z /\
-  (y <= (Zmax x y))%Z.
+Require int.Int.
+Require int.MinMax.
 
-Axiom Max_is_some : forall (x:Z) (y:Z), ((Zmax x y) = x) \/ ((Zmax x y) = y).
-
-Axiom Min_is_le : forall (x:Z) (y:Z), ((Zmin x y) <= x)%Z /\
-  ((Zmin x y) <= y)%Z.
-
-Axiom Min_is_some : forall (x:Z) (y:Z), ((Zmin x y) = x) \/ ((Zmin x y) = y).
-
-Axiom Max_x : forall (x:Z) (y:Z), (y <= x)%Z -> ((Zmax x y) = x).
-
-Axiom Max_y : forall (x:Z) (y:Z), (x <= y)%Z -> ((Zmax x y) = y).
-
-Axiom Min_x : forall (x:Z) (y:Z), (x <= y)%Z -> ((Zmin x y) = x).
-
-Axiom Min_y : forall (x:Z) (y:Z), (y <= x)%Z -> ((Zmin x y) = y).
-
-Axiom Max_sym : forall (x:Z) (y:Z), (y <= x)%Z -> ((Zmax x y) = (Zmax y x)).
-
-Axiom Min_sym : forall (x:Z) (y:Z), (y <= x)%Z -> ((Zmin x y) = (Zmin y x)).
-
+(* Why3 assumption *)
 Inductive list (a:Type) :=
   | Nil : list a
   | Cons : a -> (list a) -> list a.
-Set Contextual Implicit.
-Implicit Arguments Nil.
-Unset Contextual Implicit.
-Implicit Arguments Cons.
+Implicit Arguments Nil [[a]].
+Implicit Arguments Cons [[a]].
 
-Set Implicit Arguments.
-Fixpoint length (a:Type)(l:(list a)) {struct l}: Z :=
+(* Why3 assumption *)
+Fixpoint length {a:Type}(l:(list a)) {struct l}: Z :=
   match l with
-  | Nil  => 0%Z
-  | Cons _ r => (1%Z + (length r))%Z
+  | Nil => 0%Z
+  | (Cons _ r) => (1%Z + (length r))%Z
   end.
-Unset Implicit Arguments.
 
-Axiom Length_nonnegative : forall (a:Type), forall (l:(list a)),
+Axiom Length_nonnegative : forall {a:Type}, forall (l:(list a)),
   (0%Z <= (length l))%Z.
 
-Axiom Length_nil : forall (a:Type), forall (l:(list a)),
-  ((length l) = 0%Z) <-> (l = (Nil:(list a))).
+Axiom Length_nil : forall {a:Type}, forall (l:(list a)),
+  ((length l) = 0%Z) <-> (l = (Nil :(list a))).
 
 Parameter char : Type.
 
+(* Why3 assumption *)
 Definition word  := (list char).
 
+(* Why3 assumption *)
 Inductive dist : (list char) -> (list char) -> Z -> Prop :=
-  | dist_eps : (dist (Nil:(list char)) (Nil:(list char)) 0%Z)
+  | dist_eps : (dist (Nil :(list char)) (Nil :(list char)) 0%Z)
   | dist_add_left : forall (w1:(list char)) (w2:(list char)) (n:Z), (dist w1
       w2 n) -> forall (a:char), (dist (Cons a w1) w2 (n + 1%Z)%Z)
   | dist_add_right : forall (w1:(list char)) (w2:(list char)) (n:Z), (dist w1
@@ -59,68 +40,64 @@ Inductive dist : (list char) -> (list char) -> Z -> Prop :=
   | dist_context : forall (w1:(list char)) (w2:(list char)) (n:Z), (dist w1
       w2 n) -> forall (a:char), (dist (Cons a w1) (Cons a w2) n).
 
+(* Why3 assumption *)
 Definition min_dist(w1:(list char)) (w2:(list char)) (n:Z): Prop := (dist w1
   w2 n) /\ forall (m:Z), (dist w1 w2 m) -> (n <= m)%Z.
 
-Set Implicit Arguments.
-Fixpoint infix_plpl (a:Type)(l1:(list a)) (l2:(list a)) {struct l1}: (list
+(* Why3 assumption *)
+Fixpoint infix_plpl {a:Type}(l1:(list a)) (l2:(list a)) {struct l1}: (list
   a) :=
   match l1 with
-  | Nil  => l2
-  | Cons x1 r1 => (Cons x1 (infix_plpl r1 l2))
+  | Nil => l2
+  | (Cons x1 r1) => (Cons x1 (infix_plpl r1 l2))
   end.
-Unset Implicit Arguments.
 
-Axiom Append_assoc : forall (a:Type), forall (l1:(list a)) (l2:(list a))
+Axiom Append_assoc : forall {a:Type}, forall (l1:(list a)) (l2:(list a))
   (l3:(list a)), ((infix_plpl l1 (infix_plpl l2
   l3)) = (infix_plpl (infix_plpl l1 l2) l3)).
 
-Axiom Append_l_nil : forall (a:Type), forall (l:(list a)), ((infix_plpl l
-  (Nil:(list a))) = l).
+Axiom Append_l_nil : forall {a:Type}, forall (l:(list a)), ((infix_plpl l
+  (Nil :(list a))) = l).
 
-Axiom Append_length : forall (a:Type), forall (l1:(list a)) (l2:(list a)),
+Axiom Append_length : forall {a:Type}, forall (l1:(list a)) (l2:(list a)),
   ((length (infix_plpl l1 l2)) = ((length l1) + (length l2))%Z).
 
-Set Implicit Arguments.
-Fixpoint mem (a:Type)(x:a) (l:(list a)) {struct l}: Prop :=
+(* Why3 assumption *)
+Fixpoint mem {a:Type}(x:a) (l:(list a)) {struct l}: Prop :=
   match l with
-  | Nil  => False
-  | Cons y r => (x = y) \/ (mem x r)
+  | Nil => False
+  | (Cons y r) => (x = y) \/ (mem x r)
   end.
-Unset Implicit Arguments.
 
-Axiom mem_append : forall (a:Type), forall (x:a) (l1:(list a)) (l2:(list a)),
+Axiom mem_append : forall {a:Type}, forall (x:a) (l1:(list a)) (l2:(list a)),
   (mem x (infix_plpl l1 l2)) <-> ((mem x l1) \/ (mem x l2)).
 
-Axiom mem_decomp : forall (a:Type), forall (x:a) (l:(list a)), (mem x l) ->
+Axiom mem_decomp : forall {a:Type}, forall (x:a) (l:(list a)), (mem x l) ->
   exists l1:(list a), exists l2:(list a), (l = (infix_plpl l1 (Cons x l2))).
 
-Set Implicit Arguments.
+(* Why3 assumption *)
 Fixpoint last_char(a:char) (u:(list char)) {struct u}: char :=
   match u with
-  | Nil  => a
-  | Cons c uqt => (last_char c uqt)
+  | Nil => a
+  | (Cons c u') => (last_char c u')
   end.
-Unset Implicit Arguments.
 
-Set Implicit Arguments.
+(* Why3 assumption *)
 Fixpoint but_last(a:char) (u:(list char)) {struct u}: (list char) :=
   match u with
-  | Nil  => (Nil:(list char))
-  | Cons c uqt => (Cons a (but_last c uqt))
+  | Nil => (Nil :(list char))
+  | (Cons c u') => (Cons a (but_last c u'))
   end.
-Unset Implicit Arguments.
 
 Axiom first_last_explicit : forall (u:(list char)) (a:char),
-  ((infix_plpl (but_last a u) (Cons (last_char a u) (Nil:(list
+  ((infix_plpl (but_last a u) (Cons (last_char a u) (Nil :(list
   char)))) = (Cons a u)).
 
-(* YOU MAY EDIT THE CONTEXT BELOW *)
 
-(* DO NOT EDIT BELOW *)
 
+(* Why3 goal *)
 Theorem first_last : forall (a:char) (u:(list char)), exists v:(list char),
-  exists b:char, ((infix_plpl v (Cons b (Nil:(list char)))) = (Cons a u)) /\
+  exists b:char, ((infix_plpl v (Cons b (Nil :(list char)))) = (Cons a u)) /\
   ((length v) = (length u)).
 (* YOU MAY EDIT THE PROOF BELOW *)
 intros a u.
@@ -131,9 +108,8 @@ split.
 generalize a; induction u; intros.
 simpl; omega.
 unfold but_last; fold but_last.
-unfold length; fold length.
+unfold length; fold @length.
 generalize (IHu a0); intros; omega.
 Qed.
-(* DO NOT EDIT BELOW *)
 
 
