examples/programs/vstte12_tree_reconstruction/vstte12_tree_reconstruction_WP_Harness_WP_parameter_harness_3.v
@@ -3,90 +3,72 @@
 Require Import ZArith.
 Require Import Rbase.
 Require int.Int.
+
+(* Why3 assumption *)
 Definition unit  := unit.
 
-Parameter qtmark : Type.
-
-Parameter at1: forall (a:Type), a -> qtmark -> a.
-
-Implicit Arguments at1.
-
-Parameter old: forall (a:Type), a -> a.
-
-Implicit Arguments old.
-
-Definition implb(x:bool) (y:bool): bool := match (x,
-  y) with
-  | (true, false) => false
-  | (_, _) => true
-  end.
-
+(* Why3 assumption *)
 Inductive list (a:Type) :=
   | Nil : list a
   | Cons : a -> (list a) -> list a.
-Set Contextual Implicit.
-Implicit Arguments Nil.
-Unset Contextual Implicit.
-Implicit Arguments Cons.
+Implicit Arguments Nil [[a]].
+Implicit Arguments Cons [[a]].
 
-Set Implicit Arguments.
-Fixpoint length (a:Type)(l:(list a)) {struct l}: Z :=
-  match l with
-  | Nil => 0%Z
-  | (Cons _ r) => (1%Z + (length r))%Z
-  end.
-Unset Implicit Arguments.
-
-Axiom Length_nonnegative : forall (a:Type), forall (l:(list a)),
-  (0%Z <= (length l))%Z.
-
-Axiom Length_nil : forall (a:Type), forall (l:(list a)),
-  ((length l) = 0%Z) <-> (l = (Nil :(list a))).
-
-Set Implicit Arguments.
-Fixpoint infix_plpl (a:Type)(l1:(list a)) (l2:(list a)) {struct l1}: (list
+(* Why3 assumption *)
+Fixpoint infix_plpl {a:Type}(l1:(list a)) (l2:(list a)) {struct l1}: (list
   a) :=
   match l1 with
   | Nil => l2
   | (Cons x1 r1) => (Cons x1 (infix_plpl r1 l2))
   end.
-Unset Implicit Arguments.
 
-Axiom Append_assoc : forall (a:Type), forall (l1:(list a)) (l2:(list a))
+Axiom Append_assoc : forall {a:Type}, forall (l1:(list a)) (l2:(list a))
   (l3:(list a)), ((infix_plpl l1 (infix_plpl l2
   l3)) = (infix_plpl (infix_plpl l1 l2) l3)).
 
-Axiom Append_l_nil : forall (a:Type), forall (l:(list a)), ((infix_plpl l
+Axiom Append_l_nil : forall {a:Type}, forall (l:(list a)), ((infix_plpl l
   (Nil :(list a))) = l).
 
-Axiom Append_length : forall (a:Type), forall (l1:(list a)) (l2:(list a)),
+(* Why3 assumption *)
+Fixpoint length {a:Type}(l:(list a)) {struct l}: Z :=
+  match l with
+  | Nil => 0%Z
+  | (Cons _ r) => (1%Z + (length r))%Z
+  end.
+
+Axiom Length_nonnegative : forall {a:Type}, forall (l:(list a)),
+  (0%Z <= (length l))%Z.
+
+Axiom Length_nil : forall {a:Type}, forall (l:(list a)),
+  ((length l) = 0%Z) <-> (l = (Nil :(list a))).
+
+Axiom Append_length : forall {a:Type}, forall (l1:(list a)) (l2:(list a)),
   ((length (infix_plpl l1 l2)) = ((length l1) + (length l2))%Z).
 
-Set Implicit Arguments.
-Fixpoint mem (a:Type)(x:a) (l:(list a)) {struct l}: Prop :=
+(* Why3 assumption *)
+Fixpoint mem {a:Type}(x:a) (l:(list a)) {struct l}: Prop :=
   match l with
   | Nil => False
   | (Cons y r) => (x = y) \/ (mem x r)
   end.
-Unset Implicit Arguments.
 
-Axiom mem_append : forall (a:Type), forall (x:a) (l1:(list a)) (l2:(list a)),
+Axiom mem_append : forall {a:Type}, forall (x:a) (l1:(list a)) (l2:(list a)),
   (mem x (infix_plpl l1 l2)) <-> ((mem x l1) \/ (mem x l2)).
 
-Axiom mem_decomp : forall (a:Type), forall (x:a) (l:(list a)), (mem x l) ->
+Axiom mem_decomp : forall {a:Type}, forall (x:a) (l:(list a)), (mem x l) ->
   exists l1:(list a), exists l2:(list a), (l = (infix_plpl l1 (Cons x l2))).
 
+(* Why3 assumption *)
 Inductive tree  :=
   | Leaf : tree 
   | Node : tree -> tree -> tree .
 
-Set Implicit Arguments.
+(* Why3 assumption *)
 Fixpoint depths(d:Z) (t:tree) {struct t}: (list Z) :=
   match t with
   | Leaf => (Cons d (Nil :(list Z)))
   | (Node l r) => (infix_plpl (depths (d + 1%Z)%Z l) (depths (d + 1%Z)%Z r))
   end.
-Unset Implicit Arguments.
 
 Axiom depths_head : forall (t:tree) (d:Z), match (depths d
   t) with
@@ -98,37 +80,49 @@ Axiom depths_unique : forall (t1:tree) (t2:tree) (d:Z) (s1:(list Z))
   (s2:(list Z)), ((infix_plpl (depths d t1) s1) = (infix_plpl (depths d t2)
   s2)) -> ((t1 = t2) /\ (s1 = s2)).
 
+Axiom depths_prefix : forall (t:tree) (d1:Z) (d2:Z) (s1:(list Z)) (s2:(list
+  Z)), ((infix_plpl (depths d1 t) s1) = (infix_plpl (depths d2 t) s2)) ->
+  (d1 = d2).
+
+Axiom depths_prefix_simple : forall (t:tree) (d1:Z) (d2:Z), ((depths d1
+  t) = (depths d2 t)) -> (d1 = d2).
+
+Axiom depths_subtree : forall (t1:tree) (t2:tree) (d1:Z) (d2:Z) (s1:(list
+  Z)), ((infix_plpl (depths d1 t1) s1) = (depths d2 t2)) -> (d2 <= d1)%Z.
+
+Axiom depths_unique2 : forall (t1:tree) (t2:tree) (d1:Z) (d2:Z), ((depths d1
+  t1) = (depths d2 t2)) -> ((d1 = d2) /\ (t1 = t2)).
+
+(* Why3 assumption *)
 Definition lex(x1:((list Z)* Z)%type) (x2:((list Z)* Z)%type): Prop :=
   match x1 with
   | (s1, d1) =>
       match x2 with
-      | (s2, d2) => ((length s1) <  (length s2))%Z \/
+      | (s2, d2) => ((length s1) < (length s2))%Z \/
           (((length s1) = (length s2)) /\ match (s1,
           s2) with
-          | ((Cons h1 _), (Cons h2 _)) => ((d2 <  d1)%Z /\ (d1 <= h1)%Z) /\
+          | ((Cons h1 _), (Cons h2 _)) => ((d2 < d1)%Z /\ (d1 <= h1)%Z) /\
               (h1 = h2)
           | _ => False
           end)
       end
   end.
 
-(* YOU MAY EDIT THE CONTEXT BELOW *)
 
-(* DO NOT EDIT BELOW *)
 
+(* Why3 goal *)
 Theorem WP_parameter_harness : forall (result:tree), ((depths 0%Z
   result) = (Cons 1%Z (Cons 3%Z (Cons 3%Z (Cons 2%Z (Nil :(list Z))))))) ->
   (result = (Node Leaf (Node (Node Leaf Leaf) Leaf))).
 (* YOU MAY EDIT THE PROOF BELOW *)
 intuition.
 
-rewrite <- (Append_l_nil _ (depths 0 result)) in H.
-rewrite <- (Append_l_nil _ (Cons 1%Z (Cons 3%Z (Cons 3%Z (Cons 2%Z Nil))))) in H.
+rewrite <- (Append_l_nil (depths 0 result)) in H.
+rewrite <- (Append_l_nil (Cons 1%Z (Cons 3%Z (Cons 3%Z (Cons 2%Z Nil))))) in H.
 replace (Cons 1%Z (Cons 3%Z (Cons 3%Z (Cons 2%Z Nil)))) with
    (depths 0 (Node Leaf (Node (Node Leaf Leaf) Leaf))) in H by reflexivity.
 generalize (depths_unique _ _ _ _ _ H); intuition.
 
 Qed.
-(* DO NOT EDIT BELOW *)
 
 
